fix ident conflict

test/c/c2rust/test.c
@@ -1,5 +1,5 @@
 
-#include <stdio.h>
+// #include <stdio.h>
 int f(int a){
   int b = a-1;
   if(a>1){
@@ -11,7 +11,7 @@ int f(int a){
 }
 int main() {
   int a = 5;
-  a ^= f(a);
-  printf("Factorial of %d is %d\n", a, a);
+  // a ^= f(a);
+  // printf("Factorial of %d is %d\n", a, a);
   return 0;
 }
